Phi_Semantics/PhiSem_Mem_C.thy
@@ -214,29 +214,32 @@ proc op_free_mem:
  
 declare [[\<phi>trace_reasoning = 0]]
 
-\<phi>type_def Mem_Slice :: \<open>logaddr \<Rightarrow> nat \<Rightarrow> nat \<Rightarrow> (mem_fic,'a) \<phi> \<Rightarrow> (fiction, 'a list) \<phi>\<close> ("\<s>\<l>\<i>\<c>\<e>[_, _ : _]")
-  where \<open>l \<Ztypecolon> \<s>\<l>\<i>\<c>\<e>[addr, start : len] T \<equiv> zip [start..<start+len] l \<Ztypecolon> \<big_ast> \<lbrakk>start : len\<rwpar> (\<Sigma> j. \<m>\<e>\<m>[addr \<tribullet>\<^sub>a j\<^sup>\<t>\<^sup>\<h>] T) \<s>\<u>\<b>\<j> length l = len\<close>
+\<phi>type_def Mem_Slice :: \<open>logaddr \<Rightarrow> nat len_intvl \<Rightarrow> (mem_fic,'a) \<phi> \<Rightarrow> (fiction, 'a list) \<phi>\<close>
+  where \<open>l \<Ztypecolon> Mem_Slice addr iv T \<equiv>
+          zip [len_intvl.start iv ..< len_intvl.start iv + len_intvl.len iv] l
+            \<Ztypecolon> \<big_ast>\<^sub>\<lbrakk>\<^sub>:\<^sub>\<rbrakk>\<^sup>\<phi> iv (\<Sigma> j. \<m>\<e>\<m>[addr \<tribullet>\<^sub>a j\<^sup>\<t>\<^sup>\<h>] T) \<s>\<u>\<b>\<j> length l = len_intvl.len iv\<close>
     \<comment> \<open>Length is still required because it determines the domain of the \<phi>-type so guides the reasoning\<close>
   deriving Sep_Functor_1
        and \<open>Abstract_Domain T P
-        \<Longrightarrow> Abstract_Domain (\<s>\<l>\<i>\<c>\<e>[addr, start : len] T) (\<lambda>x. length x = len \<and> list_all P x) \<close>
-            tactic: (simp add: list_all_length)
+        \<Longrightarrow> Abstract_Domain (Mem_Slice addr iv T) (\<lambda>x. length x = len_intvl.len iv \<and> list_all P x) \<close>
+            tactic: (cases iv; simp add: list_all_length)
        and \<open>Object_Equiv T eq
-        \<Longrightarrow> Object_Equiv (\<s>\<l>\<i>\<c>\<e>[addr, start : len] T) (list_all2 eq) \<close>
+        \<Longrightarrow> Object_Equiv (Mem_Slice addr iv T) (list_all2 eq) \<close>
             tactic: (simp add: list_all2_conv_all_nth)
        and \<open>Identity_Elements\<^sub>I T T\<^sub>D T\<^sub>P
-        \<Longrightarrow> Identity_Elements\<^sub>I (\<s>\<l>\<i>\<c>\<e>[addr, start : len] T) (list_all T\<^sub>D) (\<lambda>x. length x = len \<and> list_all T\<^sub>P x) \<close>
+        \<Longrightarrow> Identity_Elements\<^sub>I (Mem_Slice addr iv T) (list_all T\<^sub>D) (\<lambda>x. length x = len_intvl.len iv \<and> list_all T\<^sub>P x) \<close>
        and \<open>Identity_Elements\<^sub>E T T\<^sub>D
-        \<Longrightarrow> Identity_Elements\<^sub>E (\<s>\<l>\<i>\<c>\<e>[addr, start : len] T) (\<lambda>x. length x = len \<and> list_all T\<^sub>D x) \<close>
+        \<Longrightarrow> Identity_Elements\<^sub>E (Mem_Slice addr iv T) (\<lambda>x. length x = len_intvl.len iv \<and> list_all T\<^sub>D x) \<close>
        and Transformation_Functor
            tactic: (auto simp add: in_set_conv_nth list_all2_conv_all_nth list_all_length ;
                     subgoal' for r l la lc \<open>rule exI[where x=\<open>map snd lc\<close>]\<close>)
-       and \<open>Separation_Homo\<^sub>I \<s>\<l>\<i>\<c>\<e>[addr, start : len] \<s>\<l>\<i>\<c>\<e>[addr, start : len] \<s>\<l>\<i>\<c>\<e>[addr, start : len] T U UNIV zip' \<close>
+       and \<open>Separation_Homo\<^sub>I (Mem_Slice addr iv) (Mem_Slice addr iv) (Mem_Slice addr iv) T U UNIV zip' \<close>
             tactic: (clarsimp simp add: list_all2_conv_all_nth zip'_def in_set_conv_nth)
        and Separation_Homo\<^sub>E
             tactic: (clarsimp simp add: list_all2_conv_all_nth unzip'_def)
+       (*and Semimodule_SDistr_Homo\<^sub>Z*)
 
-term \<open>Semimodule_SDistr_Homo\<^sub>Z \<close>
+term \<open>Semimodule_SDistr_Homo\<^sub>Z (Mem_Slice addr) T (\<lambda>_. True) \<close>
 
 
 term \<open>Separation_Homo\<^sub>E \<s>\<l>\<i>\<c>\<e>[addr, start : len] \<s>\<l>\<i>\<c>\<e>[addr, start : len] \<s>\<l>\<i>\<c>\<e>[addr, start : len] T U\<close>
